liveness.v
@@ -64,8 +64,8 @@ unfold once_until in |- *; unfold is_followed in |- *;
 intros P Q str H_always H_P.
 inversion H_always.
 apply until_eventually with (P := P).
-apply H.
-rewrite H1; assumption.
+apply C_always3.
+(*rewrite H1;*) assumption.
 Qed.
 
 Lemma followed_until :
@@ -96,7 +96,7 @@ Lemma eventually_until :
 intros P str dec; simple induction 1; clear H str.
 intros str H_P; constructor 1; assumption.
 intros s str H_ev H_until.
-elim (dec (cons_str s str)); intro H_P.
+elim (dec (Conn s str)); intro H_P.
 constructor 1; assumption.
 constructor 2; assumption.
 Qed.
@@ -118,10 +118,10 @@ unfold fairstr in |- *; unfold infinitely_often in |- *;
  unfold leads_to in |- *.
 intros P Q H_enabled leads_P_Q str H_trace H_fair H_P; generalize H_trace H_P.
 inversion_clear H_fair.
-clear H_trace H_P H0 str.
-elim H; clear H.
+clear H_trace H_P C_always4 (*str*).
+elim C_always3; clear C_always3.
 
-clear s0 str0; intro str; case str. 
+(*clear s0 str0;*)clear str. intro str; case str. 
 clear str; intros s str H_fair H_trace H_P; constructor 2; auto.
 constructor 1; unfold state2stream_formula in |- *;
  apply leads_P_Q with (s := s); auto.
@@ -131,11 +131,11 @@ apply H_enabled; auto.
 unfold state2stream_formula in |- *; simpl in |- *;
  intros s1 str1 H_ind H1 H_trace H_P.
 inversion_clear H_trace.
-inversion H.
+inversion C_always3.
 constructor 2; auto.
 apply H1; auto.
-simpl in H2; rewrite <- H2; assumption.
-simpl in H2; constructor 2; auto.
+simpl in H. rewrite <- H; assumption.
+simpl in H; constructor 2; auto.
 constructor 1; apply leads_P_Q with (s := s1); trivial.
 Qed.
 
